checker/theories/Closed.v
@@ -553,13 +553,13 @@ Proof.
     unfold test_def. simpl. rtoProp.
     split.
     rewrite -> app_context_length in *. rewrite -> Nat.add_comm in *.
-    eapply closedn_lift_inv in H2; eauto. lia.
+    eapply closedn_lift_inv in H3; eauto. lia.
     subst types.
-    now rewrite -> app_context_length, fix_context_length in H1.
-    eapply (nth_error_all) in H; eauto. simpl in *.
+    now rewrite -> app_context_length, fix_context_length in H2.
+    eapply (nth_error_all) in H0; eauto. simpl in *.
     intuition. rtoProp.
-    subst types. rewrite app_context_length Nat.add_comm in H1.
-    now eapply closedn_lift_inv in H1.
+    subst types. rewrite app_context_length Nat.add_comm in H2.
+    now eapply closedn_lift_inv in H2.
 Qed.
 
 Lemma declared_decl_closed `{checker_flags} {Σ : global_env} {cst decl} :
